{
  "cells": [
    {
      "cell_type": "markdown",
      "id": "7ffd39cf-9e03-4e0f-91d1-d74baf9aafc2",
      "metadata": {},
      "source": [
        "# Normal Forms and Transformations in Context-Free Grammars\n",
        "\n",
        "## Introduction\n",
        "\n",
        "This chapter explores various normal forms and transformations in context-free grammars (CFGs). We will discuss algorithms to convert grammars into different normal forms and demonstrate their properties through examples.\n"
      ]
    },
    {
      "cell_type": "markdown",
      "id": "8301fd3f-ca9a-471a-9b6c-88b531637584",
      "metadata": {},
      "source": [
        "## 1. Regular Grammar\n",
        "\n",
        "### 1.1 Regular Grammar Definition:\n",
        "\n",
        "A regular grammar is a special type of context-free grammar where production rules follow specific patterns. In a regular grammar, all productions must be in one of these forms:\n",
        "- $A → xB$ (where A, B are single non-terminals and x is a string of terminals, x can be empty)\n",
        "- $A → x$ (where A is a single non-terminal and x is a string of terminals, x can be empty)\n",
        "\n",
        "### 1.2 Regular Grammar Examples:\n",
        "\n",
        "#### Example 1: Regular Grammar\n",
        "Given this Grammar:\n",
        "- V: {S, A}\n",
        "- $\\Sigma$: {a, b}\n",
        "- R: $\\{S → aA | bB | a; A → aA | bA | ∧\\}$\n",
        "\n",
        "This is a regular grammar because each production follows the specific patterns outlined for a regular grammar.\n",
        "\n",
        "#### Example 2: Regular Grammar\n",
        "Given this Grammar:\n",
        "- V: {S, A, B}\n",
        "- $\\Sigma$: {a, b}\n",
        "- R: $\\{S → A | ∧; A → aB; B → aA | bB | b\\}$\n",
        "\n",
        "This is a regular grammar because each production follows the specific patterns outlined for a regular grammar.\n",
        "\n",
        "### 1.3 Regular Grammar to Regular Expression:\n",
        "Regular grammars are equivalent in power to regular expressions. Any language that can be described by a regular expression can also be described by a regular grammar, and vice versa. \n",
        "\n",
        "#### Example 3: Regular Grammar to Regular Expression\n",
        "Given the regular grammar:\n",
        "- V: {S}\n",
        "- $\\Sigma$: {a, b}\n",
        "- R: $\\{S → aS | b\\}$\n",
        "\n",
        "This CFG corresponds to the regular expression **aa*b**, because the **aa\\*** means one or more occurrences of 'a' and is followed by 'b'.\n",
        "\n",
        "#### Example 4: Regular Grammar to Regular Expression\n",
        "Given the regular grammar:\n",
        "- V: {S}\n",
        "- $\\Sigma$: {a, b}\n",
        "- R: $\\{S → abS | baS | ∧\\}$\n",
        "\n",
        "This is a regular grammar because each production follows the specific patterns outlined for a regular grammar. We can observe that every string generated by this grammar will consist of any number of occurrences of the substrings \"ab\" and \"ba\" concatenated in some order, and the production S → ∧ allows us to stop the derivation and terminate with the empty string. The language generated by this grammar consists of strings that can be a finite sequence of the substrings \"ab\" and \"ba\" (the strings consist of any number of \"ab\"s and \"ba\"s in any order). Thus, it can be expressed by the regular expression: **(ab + ba)\\***."
      ]
    },
    {
      "cell_type": "markdown",
      "id": "f515f922-3239-4127-a920-6612c397797f",
      "metadata": {},
      "source": [
        "### 1.4 Finite Automata to Regular Grammar:\n",
        "Regular grammars have a direct correspondence with finite automata. In a regular grammar, non-terminals correspond to states in the automaton, productions correspond to transitions, terminal productions correspond to accepting states, and the start symbol corresponds to the initial state. Let's look at some examples of converting between finite automata and regular grammars:\n",
        "\n",
        "#### Example 5: Finite Automaton to Regular Grammar\n",
        "Given this FA:\n",
        "```{mermaid}\n",
        "stateDiagram-v2\n",
        "    accTitle: Example 5: Finite Automaton to Regular Grammar\n",
        "    accDescr: a diagram representing a Finite Automaton\n",
        "    direction LR\n",
        "    [*] --> S\n",
        "    S --> S : 0\n",
        "    S --> A : 1\n",
        "    A --> S : 1\n",
        "    A --> F : 0\n",
        "    F --> S : 1\n",
        "    F --> F : 0\n",
        "    \n",
        "    note right of F: Accept State\n",
        "```\n",
        "\n",
        "From the given finite automaton (FA), we follow this approach to convert it to a regular grammar:\n",
        "* Ceate a non-terminal symbol for each state in the FA. In this example, we have V: {S, A, F}\n",
        "* Create a terminal symbol for each transition label in the FA. In this example, we have $\\Sigma$: {0, 1}\n",
        "* For each transition **$\\delta$(q, a) = p** in the FA, where **q** is the current state, **a** is the input symbol, and **p** is the next state,\n",
        "  - if **p** is an accept state, add productions: Q → aP | a;\n",
        "  - if **p** is not an accept state, add production: Q → aP  \n",
        "  In this example, we add productions: S → 0S | 1A; A → 1S | 0F; F → 0F | 1S. Because F is an accept state, we rewrite the productions as follows:\n",
        "  S → 0S | 1A; A → 1S | 0F | 0; F → 0F | 1S | 0\n",
        "* The start symbol of the grammar is the non-terminal corresponding to the initial state.\n",
        "\n",
        "#### Example 6: Finite Automaton to Regular Grammar\n",
        "Given this FA:\n",
        "```{mermaid}\n",
        "stateDiagram-v2\n",
        "    accTitle: Example 6: Finite Automaton to Regular Grammar\n",
        "    accDescr: a diagram representing a Finite Automaton\n",
        "    direction LR\n",
        "    [*] --> E\n",
        "    E --> E : 0\n",
        "    E --> F : 1\n",
        "    F --> F : 0\n",
        "    F --> E : 1\n",
        "    \n",
        "    note right of F: Accept State\n",
        "```\n",
        "\n",
        "From the given finite automaton (FA), we follow the approach discussed in the previous example to convert it to a regular grammar:\n",
        "* V: {S, E, F}\n",
        "* $\\Sigma$: {0, 1}\n",
        "* R: {S → E; E → 0E | 1F | 1;  F → 0F | 1E | 0}\n",
        "\n",
        "#### Example 7: Finite Automaton to Regular Grammar\n",
        "Given this FA:\n",
        "```{mermaid}\n",
        "stateDiagram-v2\n",
        "    accTitle: Example 7: Finite Automaton to Regular Grammar\n",
        "    accDescr: a diagram representing a Finite Automaton\n",
        "    direction LR\n",
        "    [*] --> S\n",
        "    S --> S : b\n",
        "    S --> A : a\n",
        "    A --> A : a\n",
        "    A --> B : b\n",
        "    B --> S : a\n",
        "    B --> F : b\n",
        "    F --> S : b\n",
        "    F --> A : a\n",
        "    \n",
        "    note right of F: Accept State\n",
        "```\n",
        "\n",
        "From the given finite automaton (FA), we follow the approach discussed in the previous example to convert it to a regular grammar:\n",
        "* V: {S, A, B, F}\n",
        "* $\\Sigma$: {a, b}\n",
        "* R: {S → bS | aA; A → aA | bB; B → aS | bF | b; F → bS | aA}\n",
        "\n",
        "### 1.5 Example Python Implementation"
      ]
    },
    {
      "cell_type": "code",
      "execution_count": 1,
      "id": "02a9dc0c-5838-4b36-b2bb-fe501f38d72f",
      "metadata": {},
      "outputs": [],
      "source": [
        "# code to define context-free grammar and productions necessary for the following sections\n",
        "class Production:\n",
        "    def __init__(self, left, right):\n",
        "        self.left = left  # Left-hand side (non-terminal)\n",
        "        self.right = right  # Right-hand side (string of terminals and non-terminals)\n",
        "    \n",
        "    def __str__(self):\n",
        "        return f\"{self.left} → {''.join(self.right)}\"\n",
        "\n",
        "class Grammar:\n",
        "    def __init__(self, productions, start_symbol):\n",
        "        self.productions = productions\n",
        "        self.start_symbol = start_symbol\n",
        "        self.terminals = self._find_terminals()\n",
        "        self.non_terminals = self._find_non_terminals()\n",
        "    \n",
        "    def _find_terminals(self):\n",
        "        terminals = set()\n",
        "        for prod in self.productions:\n",
        "            for symbol in prod.right:\n",
        "                if symbol.islower() or not symbol.isalpha():\n",
        "                    terminals.add(symbol)\n",
        "        return terminals\n",
        "    \n",
        "    def _find_non_terminals(self):\n",
        "        non_terminals = {self.start_symbol}\n",
        "        for prod in self.productions:\n",
        "            non_terminals.add(prod.left)\n",
        "            for symbol in prod.right:\n",
        "                if symbol.isupper():\n",
        "                    non_terminals.add(symbol)\n",
        "        return non_terminals\n",
        "    \n",
        "    def __str__(self):\n",
        "        return '\\n'.join(str(prod) for prod in self.productions)"
      ]
    },
    {
      "cell_type": "markdown",
      "id": "0b014d2f-37d9-48de-9737-ac7173af9305",
      "metadata": {},
      "source": [
        "## 2. Removing Null Productions\n",
        "\n",
        "### 2.1 What Are Null Productions?\n",
        "A null production (also called ∧-production) is a production of the form: A → ∧, where A is a non-terminal, and ∧ represents the empty string.\n",
        "\n",
        "### 2.2 Why Remove Null Productions?\n",
        "While these productions can be convenient for describing certain language features, removing them can simplify grammar analysis and parsing.\n",
        "\n",
        "* Simplified Parsing: Many parsing algorithms (like CYK) work better without null productions\n",
        "* Easier Analysis: Grammar properties become easier to analyze without null productions\n",
        "* Prerequisite for Normal Forms: Converting to Chomsky Normal Form or Greibach Normal Form requires eliminating null productions\n",
        "\n",
        "### 2.3 Important Properties\n",
        "* Removing null productions preserves the language defined by the grammar. The only exception is if the original language includes the empty string as a valid word; in that case, the empty string will be omitted from the new grammar, and we can handle this special case separately.\n",
        "* The process of removing null productions may increase the number of productions in the grammar\n",
        "* The resulting grammar generates exactly the same non-empty strings as the original grammar\n",
        "\n",
        "### 2.4 Steps to Remove Null Productions\n",
        "Follow these steps to remove null productions from a context-free grammar (CFG):\n",
        "1. Find Nullable Non-terminals:\n",
        "    - Mark all non-terminals A's with direct productions A → ∧\n",
        "    - Iteratively mark any non-terminal A whose right-hand side consists entirely of nullable symbols, such non-terminal has indirect null productions\n",
        "    - Continue until no more non-terminals can be marked nullable\n",
        "2. Generate New Productions:\n",
        "    - For each production A → X₁X₂...Xₙ\n",
        "    - Create new productions by omitting nullable symbols in all possible combinations\n",
        "    - Exclude any original and resulting null productions\n",
        "\n",
        "### 2.5 Examples to Remove Null Productions\n",
        "These following examples demonstrate various scenarios you might encounter when removing null productions, from simple cases to more complex ones involving multiple nullable symbols and nested dependencies. \n",
        "\n",
        "#### Example 1: Grammar with One Nullable Non-terminal\n",
        "Consider this grammar:\n",
        "```\n",
        "S → AB\n",
        "A → aA | ∧\n",
        "B → b\n",
        "```\n",
        "Step 1: Find nullable non-terminals: \n",
        "- A → ∧ directly, so A is nullable.\n",
        "- No other nullable symbols found.  \n",
        "\n",
        "Step 2: Generate new productions: From S → AB, since A is nullable, generate the following new productions:  \n",
        "- S → B (removing A from AB since A is nullable) \n",
        "- A → a (removing A from aA since A is nullable)\n",
        "Keep all other non-null productions.\n",
        "\n",
        "Final grammar:\n",
        "```\n",
        "S → AB | B\n",
        "A → aA | a\n",
        "B → b\n",
        "```\n",
        "\n",
        "#### Example 2: Grammar with Multiple Nullable Non-terminals\n",
        "Consider this grammar:\n",
        "```\n",
        "S → ABC\n",
        "A → aA | ∧\n",
        "B → bB | ∧\n",
        "C → c\n",
        "```\n",
        "Step 1: Find nullable non-terminals: \n",
        "- A → ∧ directly, so A is nullable.\n",
        "- B → ∧ directly, so B is nullable.\n",
        "   \n",
        "Step 2: Generate new productions: \n",
        "* From S → ABC, generate all combinations with nullable A and B:\n",
        "  - S → BC (removing A from ABC since A is nullable) \n",
        "  - S → AC (removing B from ABC since B is nullable)\n",
        "  - S → C (removing both A and B from ABC since A and B are nullable)\n",
        "* From A → aA | ∧, generate all combinations with nullable A:\n",
        "  - A → a (removing A from aA since A is nullable) \n",
        "* From B → bB | ∧, generate all combinations with nullable B:\n",
        "  - B → b (removing B from bB since B is nullable) \n",
        "* Keep all other non-null productions.\n",
        "\n",
        "Final grammar:\n",
        "```\n",
        "S → ABC | BC | AC | C\n",
        "A → aA | a\n",
        "B → bB | b\n",
        "C → c\n",
        "```\n",
        "\n",
        "#### Example 3: Complex Grammar with Chain of Nullable Non-terminals\n",
        "Consider this grammar:\n",
        "```\n",
        "S → AB\n",
        "A → CD\n",
        "B → b\n",
        "C → c | ∧\n",
        "D → d | ∧\n",
        "```\n",
        "Step 1: Find nullable non-terminals: \n",
        "- C → ∧ directly, so C is nullable.\n",
        "- D → ∧ directly, so D is nullable.\n",
        "- Check combinations: since CD can be null, confirming A is nullable, in other words, A can indirectly produce an empty string\n",
        "   \n",
        "Step 2: Generate new productions: \n",
        "* From A → CD, generate all combinations with nullable C and D:\n",
        "  - A → C (removing D from CD since D is nullable) \n",
        "  - A → D (removing C from CD since C is nullable)\n",
        "* From S → AB, generate all combinations with nullable A:\n",
        "  - S → B (removing A from AB since A is nullable) \n",
        "* Keep all other non-null productions.\n",
        "\n",
        "Final grammar:\n",
        "```\n",
        "S → AB | B\n",
        "A → CD | C | D\n",
        "B → b\n",
        "C → c\n",
        "D → d\n",
        "```\n",
        "\n",
        "### 2.6 Example Python Implementation"
      ]
    },
    {
      "cell_type": "code",
      "execution_count": 2,
      "id": "616e33b3-a4a9-451e-a484-00ca29596f1c",
      "metadata": {
        "editable": true,
        "slideshow": {
          "slide_type": ""
        },
        "tags": []
      },
      "outputs": [
        {
          "name": "stdout",
          "output_type": "stream",
          "text": [
            "Example 1: Simple grammar with nullable A\n",
            "Original grammar:\n",
            "S → AB\n",
            "A → aA\n",
            "A → ∧\n",
            "B → b\n",
            "\n",
            "After removing null productions:\n",
            "Nullable symbols: {'A'}\n",
            "S → AB\n",
            "S → B\n",
            "A → aA\n",
            "A → a\n",
            "B → b\n",
            "\n",
            "Analysis of transformation:\n",
            "Number of productions: 4 → 5\n",
            "Production increase factor: 1.25x\n",
            "Warning: Terminal symbols changed during transformation!\n",
            "Original terminals: {'a', '∧', 'b'}\n",
            "New terminals: {'a', 'b'}\n",
            "\n",
            "Example 2: Complex grammar with multiple nullable symbols\n",
            "Original grammar:\n",
            "S → ABC\n",
            "A → aA\n",
            "A → ∧\n",
            "B → bB\n",
            "B → ∧\n",
            "C → c\n",
            "\n",
            "After removing null productions:\n",
            "Nullable symbols: {'A', 'B'}\n",
            "S → ABC\n",
            "S → BC\n",
            "S → AC\n",
            "S → C\n",
            "A → aA\n",
            "A → a\n",
            "B → bB\n",
            "B → b\n",
            "C → c\n",
            "\n",
            "Analysis of transformation:\n",
            "Number of productions: 6 → 9\n",
            "Production increase factor: 1.50x\n",
            "Warning: Terminal symbols changed during transformation!\n",
            "Original terminals: {'a', '∧', 'b', 'c'}\n",
            "New terminals: {'a', 'b', 'c'}\n"
          ]
        }
      ],
      "source": [
        "# Sample implementation of removing null productions\n",
        "def find_nullable_symbols(grammar):\n",
        "    \"\"\"Find all nullable non-terminals in the grammar.\"\"\"\n",
        "    nullable = set()\n",
        "    changed = True\n",
        "    \n",
        "    # Keep iterating until no new nullable symbols are found\n",
        "    while changed:\n",
        "        changed = False\n",
        "        for prod in grammar.productions:\n",
        "            if prod.left not in nullable:\n",
        "                # Direct null production\n",
        "                if len(prod.right) == 1 and prod.right[0] == '∧':\n",
        "                    nullable.add(prod.left)\n",
        "                    changed = True\n",
        "                # Production with all nullable symbols\n",
        "                elif all(symbol in nullable for symbol in prod.right):\n",
        "                    nullable.add(prod.left)\n",
        "                    changed = True\n",
        "    \n",
        "    return nullable\n",
        "\n",
        "def remove_null_productions(grammar):\n",
        "    \"\"\"Remove null productions from a grammar while preserving the language.\"\"\"\n",
        "    # Step 1: Find all nullable symbols\n",
        "    nullable = find_nullable_symbols(grammar)\n",
        "    print(f\"Nullable symbols: {nullable}\")\n",
        "    \n",
        "    # Step 2: Generate new productions\n",
        "    new_productions = []\n",
        "    for prod in grammar.productions:\n",
        "        # Skip direct null productions (we'll handle start symbol separately)\n",
        "        if len(prod.right) == 1 and prod.right[0] == '∧':\n",
        "            continue\n",
        "        \n",
        "        # Generate all possible combinations of nullable symbols\n",
        "        from itertools import combinations\n",
        "        right = prod.right\n",
        "        nullable_positions = [i for i, symbol in enumerate(right) if symbol in nullable]\n",
        "        \n",
        "        for r in range(len(nullable_positions) + 1):\n",
        "            for pos_to_remove in combinations(nullable_positions, r):\n",
        "                new_right = [sym for i, sym in enumerate(right) if i not in pos_to_remove]\n",
        "                if new_right:  # Don't add empty productions unless it's for start symbol\n",
        "                    new_productions.append(Production(prod.left, new_right))\n",
        "    \n",
        "    # Step 3: Handle empty string if start symbol is nullable\n",
        "    if grammar.start_symbol in nullable:\n",
        "        new_start = f\"{grammar.start_symbol}'\"\n",
        "        new_productions.append(Production(new_start, [grammar.start_symbol]))\n",
        "        new_productions.append(Production(new_start, ['∧']))\n",
        "        return Grammar(new_productions, new_start)\n",
        "    \n",
        "    return Grammar(new_productions, grammar.start_symbol)\n",
        "\n",
        "\n",
        "# Helper function to analyze the impact of null production removal\n",
        "def analyze_grammar_transformation(original, transformed):\n",
        "    \"\"\"Analyze the changes made during null production removal.\"\"\"\n",
        "    original_prods = len(original.productions)\n",
        "    transformed_prods = len(transformed.productions)\n",
        "    \n",
        "    print(f\"Number of productions: {original_prods} → {transformed_prods}\")\n",
        "    print(f\"Production increase factor: {transformed_prods/original_prods:.2f}x\")\n",
        "    \n",
        "    # Analyze which non-terminals were affected\n",
        "    original_nt = {prod.left for prod in original.productions}\n",
        "    transformed_nt = {prod.left for prod in transformed.productions}\n",
        "    \n",
        "    new_nt = transformed_nt - original_nt\n",
        "    if new_nt:\n",
        "        print(f\"New non-terminals added: {new_nt}\")\n",
        "    \n",
        "    # Check for preservation of terminals\n",
        "    original_terms = original.terminals\n",
        "    transformed_terms = transformed.terminals\n",
        "    \n",
        "    if original_terms != transformed_terms:\n",
        "        print(\"Warning: Terminal symbols changed during transformation!\")\n",
        "        print(f\"Original terminals: {original_terms}\")\n",
        "        print(f\"New terminals: {transformed_terms}\")\n",
        "\n",
        "# Example 1: Simple grammar with null productions\n",
        "simple_grammar = Grammar([\n",
        "    Production('S', ['A', 'B']),\n",
        "    Production('A', ['a', 'A']),\n",
        "    Production('A', ['∧']),\n",
        "    Production('B', ['b']),\n",
        "], 'S')\n",
        "\n",
        "print(\"Example 1: Simple grammar with nullable A\")\n",
        "print(\"Original grammar:\")\n",
        "print(simple_grammar)\n",
        "print(\"\\nAfter removing null productions:\")\n",
        "transformed = remove_null_productions(simple_grammar)\n",
        "print(transformed)\n",
        "print(\"\\nAnalysis of transformation:\")\n",
        "analyze_grammar_transformation(simple_grammar, transformed)\n",
        "\n",
        "# Example 2: More complex grammar with multiple nullable symbols\n",
        "complex_grammar = Grammar([\n",
        "    Production('S', ['A', 'B', 'C']),\n",
        "    Production('A', ['a', 'A']),\n",
        "    Production('A', ['∧']),\n",
        "    Production('B', ['b', 'B']),\n",
        "    Production('B', ['∧']),\n",
        "    Production('C', ['c']),\n",
        "], 'S')\n",
        "\n",
        "print(\"\\nExample 2: Complex grammar with multiple nullable symbols\")\n",
        "print(\"Original grammar:\")\n",
        "print(complex_grammar)\n",
        "print(\"\\nAfter removing null productions:\")\n",
        "transformed = remove_null_productions(complex_grammar)\n",
        "print(transformed)\n",
        "print(\"\\nAnalysis of transformation:\")\n",
        "analyze_grammar_transformation(complex_grammar, transformed)\n"
      ]
    },
    {
      "cell_type": "markdown",
      "id": "41cd74a0-cb1e-448d-a987-13ab81c02e4b",
      "metadata": {},
      "source": [
        "## 3. Removing Unit Productions\n",
        "\n",
        "### 3.1 What Are Unit Productions?\n",
        "Unit productions (also called chain productions) are productions of the form A → B where both A and B are non-terminals. While these productions can make grammars more readable and intuitive, they do not add any meaningful structure to the derivation process and can make parsing less efficient. \n",
        "\n",
        "### 3.2 Why Remove Unit Productions?\n",
        "1. Parsing Efficiency: unit productions can lead to unnecessary steps in parsing, creating longer derivation chains than needed.\n",
        "2. Grammar Analysis: many algorithms (like CYK parsing) require grammars without unit productions.\n",
        "3. Grammar Simplification: removing unit productions simplifies the grammar while preserving its language.\n",
        "\n",
        "As an example, consider this grammar for arithmetic expressions:\n",
        "```\n",
        "E → T\n",
        "T → F\n",
        "F → var\n",
        "F → num\n",
        "F → (E)\n",
        "```\n",
        "While this grammar is readable, it requires three steps (E → T → F → var) to derive a simple variable. After removing unit productions, we get:\n",
        "```\n",
        "E → var\n",
        "E → num\n",
        "E → (E)\n",
        "```\n",
        "This transformed grammar requires a single step (E → var) to derive a simple variable.\n",
        "\n",
        "### 3.3 How to Remove Unit Productions\n",
        "\n",
        "#### 3.3.1 Unit Pairs and Transitive Closure\n",
        "Before removing unit productions, we need to understand unit pairs and transitive closure. A unit pair (A,B) in a context-free grammar means that A can derive B through one or more (a sequence of) unit productions. The transitive closure of unit productions ensures that if there is a sequence of unit productions leading from one non-terminal to another, we establish a direct connection between them. For example, in the grammar:\n",
        "```\n",
        "S → A\n",
        "A → B\n",
        "B → C\n",
        "C → a\n",
        "```\n",
        "Here are the steps to find all the unit pairs:\n",
        "* Start with direct unit pairs: S → A, A → B, and B → C are direct unit pairs, so we add (S,A), (A,B), (B,C) to the unit pair set.\n",
        "* Extend the pairs transitively: If (S,A) and (A,B) exist, it means S → B exists, then add (S,B) to the unit pair set. We repeat until no new pairs can be added. By extending the pairs transitively this way, We add more pairs (S,C), (A,C).\n",
        "\n",
        "So the unit pairs are (S,A), (S,B), (S,C), (A,B), (A,C), (B,C).  \n",
        "\n",
        "We can visualize unit pairs as a directed graph: solid arrows represent direct unit productions, and dashed arrows represent derived unit pairs.\n",
        "\n",
        "```{mermaid}\n",
        "graph TD\n",
        "    accTitle: unit pairs as a directed graph\n",
        "    accDescr: a diagram representing unit pairs as a directed graph\n",
        "    S[S] --> A[A]\n",
        "    A --> B[B]\n",
        "    S -.-> B[B]\n",
        "    \n",
        "    style S fill:#f9f,stroke:#333\n",
        "    style A fill:#ff9,stroke:#333\n",
        "    style B fill:#9f9,stroke:#333\n",
        "```\n",
        "\n",
        "#### 3.3.2 Steps to Remove Unit Productions\n",
        "The process of removing unit productions involves three main steps. Let's examine each step in detail with examples.\n",
        "* Step 1. Find all unit pairs\n",
        "* Step 2. Create new productions based on all unit pairs: for each unit pair (A,B), look at all non-unit productions with B on the left side, create new productions by replacing B with A\n",
        "* Step 3. Remove original unit productions: identify all unit productions and remove them from the grammar; keep all new productions created in Step 2\n",
        "\n",
        "### 3.4 Examples to Remove Unit Productions\n",
        "\n",
        "#### Example 1: Remove unit productions from the given grammar\n",
        "```\n",
        "S → A\n",
        "A → B\n",
        "B → aB | b\n",
        "```\n",
        "Step 1: find all unit pairs: (S,A), (A,B), (S,B)\n",
        "Step 2: create new productions:\n",
        "* for (S,A), we do not find any non-unit productions with A on the left side\n",
        "* for (A,B), we find two non-unit productions with B on the left side: B → aB | b\n",
        "    - from B → aB, add new production A → aB\n",
        "    - from B → b, add new production A → b\n",
        "* for (S,B), we find two non-unit productions with B on the left side: B → aB | b\n",
        "    - from B → aB, add new production S → aB\n",
        "    - from B → b, add new production S → b\n",
        "Step 3: remove all original unit productions: S → A and A → B should be removed.\n",
        "\n",
        "After removing unit productions, the grammar is transformed to:\n",
        "```\n",
        "S → aB | b\n",
        "A → aB | b\n",
        "B → aB | b\n",
        "```\n",
        "\n",
        "#### Example 2: Remove unit productions from the given grammar\n",
        "```\n",
        "E → E + T | T\n",
        "T → T * F | F\n",
        "F → v | (E)\n",
        "```\n",
        "Step 1: find all unit pairs: (E,T), (T,F), (E,F)\n",
        "Step 2: create new productions:\n",
        "* for (E,T), we find non-unit productions with T on the left side: T → T * F\n",
        "    - add new production E → T * F\n",
        "* for (T,F), we find non-unit productions with F on the left side: F → v | (E)\n",
        "    - from F → v, add new production T → v\n",
        "    - from F → (E), add new production T → (E)\n",
        "* for (E,F), we find non-unit productions with F on the left side: F → v | (E)\n",
        "    - from F → v, add new production E → v\n",
        "    - from F → (E), add new production E → (E)\n",
        "Step 3: remove all original unit productions: E → T and T → F should be removed.\n",
        "\n",
        "After removing unit productions, the grammar is transformed to:\n",
        "```\n",
        "E → E + T | T * F | v | (E)\n",
        "T → T * F | v | (E)\n",
        "F → v | (E)\n",
        "```\n",
        "\n",
        "### 3.5 Example Python Implementation"
      ]
    },
    {
      "cell_type": "code",
      "execution_count": 3,
      "id": "966a966d-e617-484b-98e2-34f4c5baa0aa",
      "metadata": {},
      "outputs": [
        {
          "name": "stdout",
          "output_type": "stream",
          "text": [
            "Original grammar:\n",
            "S → A\n",
            "A → B\n",
            "B → aB\n",
            "B → b\n",
            "\n",
            "Grammar after removing unit productions:\n",
            "B → aB\n",
            "A → aB\n",
            "S → aB\n",
            "B → b\n",
            "A → b\n",
            "S → b\n"
          ]
        }
      ],
      "source": [
        "# Sample implementation of removing unit productions\n",
        "def remove_unit_productions(grammar):\n",
        "    \"\"\"Remove unit productions from a grammar.\"\"\"\n",
        "    def find_unit_pairs():\n",
        "        pairs = set()\n",
        "        # Initial pairs (A, A) for all non-terminals\n",
        "        for A in grammar.non_terminals:\n",
        "            pairs.add((A, A))\n",
        "        \n",
        "        changed = True\n",
        "        while changed:\n",
        "            changed = False\n",
        "            for prod in grammar.productions:\n",
        "                if len(prod.right) == 1 and prod.right[0] in grammar.non_terminals:\n",
        "                    for B, C in list(pairs):\n",
        "                        if B == prod.right[0] and (prod.left, C) not in pairs:\n",
        "                            pairs.add((prod.left, C))\n",
        "                            changed = True\n",
        "        return pairs\n",
        "\n",
        "    # Find all unit pairs\n",
        "    unit_pairs = find_unit_pairs()\n",
        "    \n",
        "    # Create new productions\n",
        "    new_productions = []\n",
        "    for prod in grammar.productions:\n",
        "        if len(prod.right) == 1 and prod.right[0] in grammar.non_terminals:\n",
        "            continue  # Skip unit productions\n",
        "        \n",
        "        for A, B in unit_pairs:\n",
        "            if B == prod.left:\n",
        "                new_productions.append(Production(A, prod.right))\n",
        "    \n",
        "    return Grammar(new_productions, grammar.start_symbol)\n",
        "\n",
        "# Example usage\n",
        "grammar_with_unit = Grammar([\n",
        "    Production('S', ['A']),\n",
        "    Production('A', ['B']),\n",
        "    Production('B', ['a', 'B']),\n",
        "    Production('B', ['b']),\n",
        "], 'S')\n",
        "\n",
        "print(\"Original grammar:\")\n",
        "print(grammar_with_unit)\n",
        "print(\"\\nGrammar after removing unit productions:\")\n",
        "print(remove_unit_productions(grammar_with_unit))"
      ]
    },
    {
      "cell_type": "markdown",
      "id": "36241775-5fd3-4db2-b588-ad3ebbe62a51",
      "metadata": {
        "editable": true,
        "slideshow": {
          "slide_type": ""
        },
        "tags": []
      },
      "source": [
        "## 4. Chomsky Normal Form\n",
        "\n",
        "### 4.1 What is Chomsky Normal Form?\n",
        "Chomsky Normal Form (CNF) is a simplified form of context-free grammars where all productions follow specific patterns. A grammar is in CNF if and only if all productions are of the form:\n",
        "```\n",
        "A → BC (where A, B, and C are non-terminals)\n",
        "A → a (where A is a non-terminal and a is a terminal)\n",
        "```\n",
        "### 4.2 What Makes CNF Valuable?\n",
        "Chomsky Normal Form is particularly important for several reasons:\n",
        "* It simplifies parsing algorithms (especially the CYK algorithm for membership testing)\n",
        "* It makes certain proofs about context-free grammars easier, such as the Pumping Lemma for Context-free Languages\n",
        "* It provides a standardized way to represent any context-free grammar\n",
        "* It eliminates complex productions while preserving the generated language\n",
        "* It is widely used in compiler design and natural language processing (NLP) for efficient parsing techniques.\n",
        "\n",
        "### 4.3 Converting a CFG to CNF\n",
        "To convert a given CFG into CNF, follow these steps:\n",
        "* Step 1: Remove all Null Productions (previously covered in earlier sections)\n",
        "* Step 2: Remove all Unit Productions (previously covered in earlier sections)\n",
        "* Step 3: Convert Remaining Productions to CNF\n",
        "    - Step 3a: Convert long right-hand sides into CNF: replace any production with three or more non-terminals on the right-hand size with new non-terminals, and repeat until all right-hand sides have exactly two non-terminals.\n",
        "    - Step 3b: Convert terminals in mixed productions: replace  terminals in rules like A → aB  with a new non-terminal\n",
        "\n",
        "#### Example 1: Converting a CFG to CNF\n",
        "Conver the given CFG to CNF:\n",
        "```\n",
        "S → AB ∣ BCA ∣ aB\n",
        "A → AB | a\n",
        "B → b\n",
        "C → c\n",
        "```\n",
        "* Step 1: No null productions\n",
        "* Step 2: No unit productions\n",
        "* Step 3a: the production S → BCA has three non-terminals on the right-hand side:\n",
        "    - Introduce a new variable X such that: X → CA\n",
        "    - Replace S → BCA with S → BX\n",
        "* Step 3b: the production S → aB contains both a terminal (a) and a non-terminal (B). \n",
        "    - introduce a new non-terminal with a new production: Y → a\n",
        "    - replace S → aB with S → YB\n",
        "\n",
        "Final CNF grammar:\n",
        "```\n",
        "S → AB ∣ BX ∣ YB\n",
        "A → AB | a\n",
        "B → b\n",
        "C → c\n",
        "X → CA\n",
        "Y → a\n",
        "```\n",
        "You may wonder, in step 3b, we introduced a new non-terminal Y with the production Y → a, instead of using the existing production A → a for the conversion. Here is why:\n",
        "* If we had used A instead of Y, we would have replaced S → aB with S → AB. However, in the original grammar, A is already defined with its own role: A → AB | a, using A instead of Y could change the structure of the grammar, possibly affecting the language it generates. In this example, it could have introduced a new production S → ABB, which is not present in the original grammar.\n",
        "* If we directly substituted A for a, it might create ambiguity in how non-terminals are structured. By introducing Y → a, we ensure that every production strictly adheres to CNF without modifying existing non-terminals.\n",
        "\n",
        "Introducing Y ensures that the structure and meaning of the original CFG remain intact while following CNF's strict format. This is a standard transformation technique when converting CFGs to CNF. \n",
        "\n",
        "#### Example 2: Converting a CFG to CNF\n",
        "Conver the given CFG to CNF:\n",
        "```\n",
        "S → aSb | bSa | SS | A\n",
        "A → aAb | bAa | ∧\n",
        "```\n",
        "* Step 1: Remove all Null Productions\n",
        "    - identify nullable non-terminals: A, S\n",
        "    - from A → aAb | bAa, generate all combinations with nullable A: A → ab | ba\n",
        "    - from S → aSb | bSa, generate all combinations with nullable S: S → ab | ba\n",
        "\n",
        "Grammar becomes:\n",
        "```\n",
        "S → aSb | bSa | SS | A | ab | ba\n",
        "A → aAb | bAa | ab | ba\n",
        "```\n",
        "* Step 2: Remove all unit productions:\n",
        "    - Step 1. Find all unit pairs: (S,A)\n",
        "    - Step 2. Create new productions for (S,A), look at all non-unit productions with A on the left side, create new productions by replacing A with S: S → aAb | bAa | ab | ba\n",
        "    - Step 3. Remove original unit productions: keep all new productions created in Step 2\n",
        "\n",
        "Grammar becomes:\n",
        "```\n",
        "S → aSb | bSa | SS | aAb | bAa | ab | ba\n",
        "A → aAb | bAa | ab | ba\n",
        "```\n",
        "* Step 3: Convert Remaining Productions to CNF\n",
        "    - Introduce two new non-terminals X and Y such that: X → a, Y → b\n",
        "    - Grammar becomes:\n",
        "        ```\n",
        "        S → XSY | YSX | SS | XAY | YAX | XY | YX\n",
        "        A → XAY | YAX | XY | YX\n",
        "        X → a\n",
        "        Y → b\n",
        "        ```\n",
        "    - Introduce two new non-terminals B, C, D, E such that: B → XS, C → YS, D → XA, E → YA\n",
        "    - A long production such as S → XSY becomes S → BY, all other long productions can be converted to CNF\n",
        "\n",
        "Final grammar becomes:\n",
        "```\n",
        "S → BY | CX | SS | DY | EX | XY | YX\n",
        "A → DY | EX | XY | YX\n",
        "X → a\n",
        "Y → b\n",
        "B → XS\n",
        "C → YS\n",
        "D → XA\n",
        "E → YA\n",
        "```\n",
        "\n",
        "### 4.4 Example Python Implementation"
      ]
    },
    {
      "cell_type": "code",
      "execution_count": 4,
      "id": "82534dce-01e4-4140-96b5-3910904f8920",
      "metadata": {},
      "outputs": [
        {
          "name": "stdout",
          "output_type": "stream",
          "text": [
            "Original grammar:\n",
            "S → ABC\n",
            "A → aA\n",
            "B → b\n",
            "C → cAB\n",
            "\n",
            "Grammar in Chomsky Normal Form:\n",
            "Nullable symbols: set()\n",
            "X_0 → BC\n",
            "S → AX_0\n",
            "T_a → a\n",
            "A → T_aA\n",
            "B → b\n",
            "T_c → c\n",
            "X_6 → AB\n",
            "C → T_cX_6\n"
          ]
        }
      ],
      "source": [
        "def to_chomsky_normal_form(grammar):\n",
        "    \"\"\"Convert a grammar to Chomsky Normal Form.\"\"\"\n",
        "    # Step 1: Remove unit productions\n",
        "    grammar = remove_unit_productions(grammar)\n",
        "    \n",
        "    # Step 2: Remove null productions\n",
        "    grammar = remove_null_productions(grammar)\n",
        "    \n",
        "    # Step 3: Replace terminals in complex productions\n",
        "    new_productions = []\n",
        "    terminal_rules = {}  # Maps terminals to their corresponding non-terminals\n",
        "    \n",
        "    for prod in grammar.productions:\n",
        "        if len(prod.right) == 1 and prod.right[0] in grammar.terminals:\n",
        "            new_productions.append(prod)\n",
        "            continue\n",
        "            \n",
        "        new_right = []\n",
        "        for symbol in prod.right:\n",
        "            if symbol in grammar.terminals:\n",
        "                if symbol not in terminal_rules:\n",
        "                    new_non_terminal = f\"T_{symbol}\"\n",
        "                    terminal_rules[symbol] = new_non_terminal\n",
        "                    new_productions.append(Production(new_non_terminal, [symbol]))\n",
        "                new_right.append(terminal_rules[symbol])\n",
        "            else:\n",
        "                new_right.append(symbol)\n",
        "        \n",
        "        # Step 4: Break long productions\n",
        "        while len(new_right) > 2:\n",
        "            new_non_terminal = f\"X_{len(new_productions)}\"\n",
        "            new_productions.append(Production(new_non_terminal, new_right[-2:]))\n",
        "            new_right = new_right[:-2] + [new_non_terminal]\n",
        "        \n",
        "        new_productions.append(Production(prod.left, new_right))\n",
        "    \n",
        "    return Grammar(new_productions, grammar.start_symbol)\n",
        "\n",
        "# Example usage\n",
        "non_cnf_grammar = Grammar([\n",
        "    Production('S', ['A', 'B', 'C']),\n",
        "    Production('A', ['a', 'A']),\n",
        "    Production('B', ['b']),\n",
        "    Production('C', ['c', 'A', 'B']),\n",
        "], 'S')\n",
        "\n",
        "print(\"Original grammar:\")\n",
        "print(non_cnf_grammar)\n",
        "print(\"\\nGrammar in Chomsky Normal Form:\")\n",
        "print(to_chomsky_normal_form(non_cnf_grammar))"
      ]
    },
    {
      "cell_type": "markdown",
      "id": "df202d70-e4b0-47ba-9f85-ba20b9c61cb9",
      "metadata": {},
      "source": [
        "## 5. Practice Exercises\n",
        "### 5.1 Exercise 1: Regular Grammar Conversion\n",
        "Convert the following finite automaton to a regular grammar:\n",
        "```{mermaid}\n",
        "stateDiagram-v2\n",
        "    accTitle: Exercise 1: Regular Grammar Conversion\n",
        "    accDescr: a diagram representing a Finite Automaton\n",
        "    direction LR\n",
        "    [*] --> Q0\n",
        "    Q0 --> Q1 : a\n",
        "    Q0 --> Q0 : b\n",
        "    Q1 --> Q2 : b\n",
        "    Q1 --> Q1 : a\n",
        "    Q2 --> Q0 : a\n",
        "    Q2 --> Q2 : b\n",
        "    \n",
        "    note right of Q2: Accept State\n",
        "```\n",
        "   \n",
        "### 5.2 Exercise 2: Null Production Elimination\n",
        "Convert the following grammar to an equivalent one without null productions:\n",
        "```\n",
        "S → AB | CD\n",
        "A → aA | ∧\n",
        "B → bB | ∧\n",
        "C → cC | ∧\n",
        "D → d\n",
        "```\n",
        "### 5.3 Exercise 3: Unit Production Elimination\n",
        "Eliminate all unit productions from this grammar:\n",
        "```\n",
        "E → E' | T\n",
        "E' → E + T\n",
        "T → T' | F\n",
        "T' → T * F\n",
        "F → v | (E)\n",
        "```\n",
        "### 5.4 Exercise 4: CFG to CNF Conversion\n",
        "Convert the following grammar to Chomsky Normal Form:\n",
        "```\n",
        "S → ASB | ∧\n",
        "A → aAS | a\n",
        "B → SbS | A | bb\n",
        "```"
      ]
    },
    {
      "cell_type": "markdown",
      "id": "1b3d4ac9-e6fd-4e8e-bf9e-2fbcbd7e9070",
      "metadata": {},
      "source": [
        "## 6. Further Reading\n",
        "* \"Introduction to the Theory of Computation\" by Michael Sipser, Section 2.1 - Context-Free Grammars\n",
        "* \"Introduction to Computer Theory\" by Daniel I.A. Cohen, Chapter 13 - Grammatical Format\n",
        "* \"Automata Theory, Languages, and Computation\" by Hopcroft, Motwani, and Ullman, Chapter 5 - Context-Free Grammars"
      ]
    }
  ],
  "metadata": {
    "kernelspec": {
      "display_name": "Python 3 (ipykernel)",
      "language": "python",
      "name": "python3"
    },
    "language_info": {
      "codemirror_mode": {
        "name": "ipython",
        "version": 3
      },
      "file_extension": ".py",
      "mimetype": "text/x-python",
      "name": "python",
      "nbconvert_exporter": "python",
      "pygments_lexer": "ipython3",
      "version": "3.13.6"
    }
  },
  "nbformat": 4,
  "nbformat_minor": 5
}